<?xml version="1.0"?>
<rdf:RDF xmlns="https://w3id.org/def/bm2o#"
     xml:base="https://w3id.org/def/bm2o"
     xmlns:dc="http://purl.org/dc/elements/1.1/"
     xmlns:ns="http://creativecommons.org/ns#"
     xmlns:owl="http://www.w3.org/2002/07/owl#"
     xmlns:rdf="http://www.w3.org/1999/02/22-rdf-syntax-ns#"
     xmlns:xml="http://www.w3.org/XML/1998/namespace"
     xmlns:xsd="http://www.w3.org/2001/XMLSchema#"
     xmlns:qudt="http://qudt.org/schema/qudt/"
     xmlns:rdfs="http://www.w3.org/2000/01/rdf-schema#"
     xmlns:skos="http://www.w3.org/2004/02/skos/core#"
     xmlns:vann="http://purl.org/vocab/vann/"
     xmlns:terms="http://purl.org/dc/terms/"
     xmlns:schema="http://schema.org#"
     xmlns:terms1="http://purl.org/dc/terms#"
     xmlns:AnnotationVocabulary="https://spec.industrialontologies.org/ontology/core/meta/AnnotationVocabulary/">
    <owl:Ontology rdf:about="https://w3id.org/def/bm2o#">
        <owl:imports rdf:resource="https://brickschema.org/schema/1.1/Brick"/>
        <owl:imports rdf:resource="https://spec.industrialontologies.org/ontology/202301/maintenance/MaintenanceReferenceOntology/"/>
        <owl:imports rdf:resource="https://spec.industrialontologies.org/ontology/202301/maintenance/Metadatamaintenance/"/>
        <ns:license rdf:resource="https://creativecommons.org/licenses/by-sa/4.0/"/>
        <terms:contributor>Alexis Lesage</terms:contributor>
        <terms:contributor>Arnaud Doniec</terms:contributor>
        <terms:contributor>Jerry Lonlac</terms:contributor>
        <terms:contributor>Maxime Lefrançois</terms:contributor>
        <terms:contributor>Stéphane Lecoeuche</terms:contributor>
        <terms:creator>Joel Mba Kouhoue</terms:creator>
        <terms:description xml:lang="en"></terms:description>
        <terms:title xml:lang="en">bm2o (Building Maintenance Operation Ontology)</terms:title>
        <vann:preferredNamespacePrefix>bm2o</vann:preferredNamespacePrefix>
        <vann:preferredNamespaceUri rdf:datatype="http://www.w3.org/2001/XMLSchema#anyURI">https://w3id.org/def/bm2o#</vann:preferredNamespaceUri>
        <owl:versionInfo xml:lang="en">1.0</owl:versionInfo>
    </owl:Ontology>
    


    <!-- 
    ///////////////////////////////////////////////////////////////////////////////////////
    //
    // Annotation properties
    //
    ///////////////////////////////////////////////////////////////////////////////////////
     -->


    


    <!-- http://creativecommons.org/ns#license -->


    <owl:AnnotationProperty rdf:about="http://creativecommons.org/ns#license"/>
    


    <!-- http://purl.org/vocab/vann/preferredNamespacePrefix -->


    <owl:AnnotationProperty rdf:about="http://purl.org/vocab/vann/preferredNamespacePrefix"/>
    


    <!-- http://purl.org/vocab/vann/preferredNamespaceUri -->


    <owl:AnnotationProperty rdf:about="http://purl.org/vocab/vann/preferredNamespaceUri"/>
    


    <!-- 
    ///////////////////////////////////////////////////////////////////////////////////////
    //
    // Object Properties
    //
    ///////////////////////////////////////////////////////////////////////////////////////
     -->


    


    <!-- https://w3id.org/def/bm2o#hasAddress -->


    <owl:ObjectProperty rdf:about="https://w3id.org/def/bm2o#hasAddress">
        <rdfs:domain rdf:resource="https://brickschema.org/schema/1.1/Brick#Location"/>
        <rdfs:range rdf:resource="https://w3id.org/def/bm2o#Address"/>
        <rdfs:comment xml:lang="en">Physical address of a location.</rdfs:comment>
        <rdfs:label xml:lang="en">has address</rdfs:label>
    </owl:ObjectProperty>
    


    <!-- https://w3id.org/def/bm2o#hasFunction -->


    <owl:ObjectProperty rdf:about="https://w3id.org/def/bm2o#hasFunction">
        <owl:inverseOf rdf:resource="https://w3id.org/def/bm2o#isRequiredFunctionOf"/>
        <rdfs:domain rdf:resource="https://brickschema.org/schema/1.1/Brick#Equipment"/>
        <rdfs:range rdf:resource="https://spec.industrialontologies.org/ontology/maintenance/MaintenanceReferenceOntology/RequiredFunction"/>
        <rdfs:comment xml:lang="en">Required function of an equipment.</rdfs:comment>
        <rdfs:label xml:lang="en">has function</rdfs:label>
    </owl:ObjectProperty>
    


    <!-- https://w3id.org/def/bm2o#isAddressOf -->


    <owl:ObjectProperty rdf:about="https://w3id.org/def/bm2o#isAddressOf">
        <rdfs:domain rdf:resource="https://w3id.org/def/bm2o#Address"/>
        <rdfs:range rdf:resource="https://brickschema.org/schema/1.1/Brick#Location"/>
        <rdfs:comment xml:lang="en">Location having this physical address.</rdfs:comment>
        <rdfs:label xml:lang="en">is address of</rdfs:label>
    </owl:ObjectProperty>
    


    <!-- https://w3id.org/def/bm2o#isRelatedAgreementOf -->


    <owl:ObjectProperty rdf:about="https://w3id.org/def/bm2o#isRelatedAgreementOf">
        <owl:inverseOf rdf:resource="https://w3id.org/def/bm2o#relatedAgreement"/>
        <rdfs:domain rdf:resource="https://spec.industrialontologies.org/ontology/core/Core/Agreement"/>
        <rdfs:range rdf:resource="https://spec.industrialontologies.org/ontology/maintenance/MaintenanceReferenceOntology/MaintenanceWorkOrderRecord"/>
        <rdfs:comment xml:lang="en">Links an agreement to some maintenance process is is related to.</rdfs:comment>
        <rdfs:label xml:lang="en">is related agreement of</rdfs:label>
    </owl:ObjectProperty>
    


    <!-- https://w3id.org/def/bm2o#isRelatedCommercialServiceOf -->


    <owl:ObjectProperty rdf:about="https://w3id.org/def/bm2o#isRelatedCommercialServiceOf">
        <owl:inverseOf rdf:resource="https://w3id.org/def/bm2o#relatedCommercialService"/>
        <rdfs:domain rdf:resource="https://spec.industrialontologies.org/ontology/core/Core/CommercialService"/>
        <rdfs:range rdf:resource="https://spec.industrialontologies.org/ontology/core/Core/Agreement"/>
        <rdfs:comment xml:lang="en">Links a commercial service to some agreement is is related to.</rdfs:comment>
        <rdfs:label xml:lang="en">is related commercial service of</rdfs:label>
    </owl:ObjectProperty>
    


    <!-- https://w3id.org/def/bm2o#isRelatedCustomerOf -->


    <owl:ObjectProperty rdf:about="https://w3id.org/def/bm2o#isRelatedCustomerOf">
        <owl:inverseOf rdf:resource="https://w3id.org/def/bm2o#relatedCustomer"/>
        <rdfs:domain rdf:resource="https://spec.industrialontologies.org/ontology/core/Core/CustomerRole"/>
        <rdfs:range rdf:resource="https://spec.industrialontologies.org/ontology/core/Core/Agreement"/>
        <rdfs:comment xml:lang="en">Links a customer to some agreement is has signed.</rdfs:comment>
        <rdfs:label xml:lang="en">is related customer of</rdfs:label>
    </owl:ObjectProperty>
    


    <!-- https://w3id.org/def/bm2o#isRelatedMaintenanceProcessOf -->


    <owl:ObjectProperty rdf:about="https://w3id.org/def/bm2o#isRelatedMaintenanceProcessOf">
        <owl:inverseOf rdf:resource="https://w3id.org/def/bm2o#relatedMaintenanceProcess"/>
        <rdfs:domain rdf:resource="https://spec.industrialontologies.org/ontology/maintenance/MaintenanceReferenceOntology/MaintenanceProcess"/>
        <rdfs:range rdf:resource="https://spec.industrialontologies.org/ontology/maintenance/MaintenanceReferenceOntology/MaintenanceWorkOrderRecord"/>
        <rdfs:comment xml:lang="en">Links a maintenance process to its description.</rdfs:comment>
        <rdfs:label xml:lang="en">is related maintenance process of</rdfs:label>
    </owl:ObjectProperty>
    


    <!-- https://w3id.org/def/bm2o#isRelatedServiceLevelAgreementOf -->


    <owl:ObjectProperty rdf:about="https://w3id.org/def/bm2o#isRelatedServiceLevelAgreementOf">
        <owl:inverseOf rdf:resource="https://w3id.org/def/bm2o#relatedServiceLevelAgreement"/>
        <rdfs:domain rdf:resource="https://w3id.org/def/bm2o#ServiceLevelAgreement"/>
        <rdfs:range rdf:resource="https://spec.industrialontologies.org/ontology/core/Core/Agreement"/>
        <rdfs:comment xml:lang="en">Links a service level agreement to the agreement it is related to.</rdfs:comment>
        <rdfs:label xml:lang="en">is related service level agreement of</rdfs:label>
    </owl:ObjectProperty>
    


    <!-- https://w3id.org/def/bm2o#isRelatedServiceProviderOf -->


    <owl:ObjectProperty rdf:about="https://w3id.org/def/bm2o#isRelatedServiceProviderOf">
        <owl:inverseOf rdf:resource="https://w3id.org/def/bm2o#relatedServiceProvider"/>
        <rdfs:domain rdf:resource="https://spec.industrialontologies.org/ontology/core/Core/ServiceProvider"/>
        <rdfs:range rdf:resource="https://spec.industrialontologies.org/ontology/core/Core/Agreement"/>
        <rdfs:comment xml:lang="en">Links a service provider to a specific agreement.</rdfs:comment>
        <rdfs:label xml:lang="en">is related service provider of</rdfs:label>
    </owl:ObjectProperty>
    


    <!-- https://w3id.org/def/bm2o#isRequiredFunctionOf -->


    <owl:ObjectProperty rdf:about="https://w3id.org/def/bm2o#isRequiredFunctionOf">
        <rdfs:domain rdf:resource="https://spec.industrialontologies.org/ontology/maintenance/MaintenanceReferenceOntology/RequiredFunction"/>
        <rdfs:range rdf:resource="https://brickschema.org/schema/1.1/Brick#Equipment"/>
        <rdfs:comment xml:lang="en">Links some asset&apos;s function to a specific equipment</rdfs:comment>
        <rdfs:label xml:lang="en">is required function of</rdfs:label>
    </owl:ObjectProperty>
    


    <!-- https://w3id.org/def/bm2o#participatesTo -->


    <owl:ObjectProperty rdf:about="https://w3id.org/def/bm2o#participatesTo">
        <owl:inverseOf rdf:resource="https://w3id.org/def/bm2o#relatedEquipment"/>
        <rdfs:domain rdf:resource="https://brickschema.org/schema/1.1/Brick#Equipment"/>
        <rdfs:range rdf:resource="https://spec.industrialontologies.org/ontology/maintenance/MaintenanceReferenceOntology/MaintenanceProcess"/>
        <rdfs:comment xml:lang="en"></rdfs:comment>
        <rdfs:label xml:lang="en">participates to</rdfs:label>
    </owl:ObjectProperty>
    


    <!-- https://w3id.org/def/bm2o#relatedAgreement -->


    <owl:ObjectProperty rdf:about="https://w3id.org/def/bm2o#relatedAgreement">
        <rdfs:domain rdf:resource="https://spec.industrialontologies.org/ontology/maintenance/MaintenanceReferenceOntology/MaintenanceWorkOrderRecord"/>
        <rdfs:range rdf:resource="https://spec.industrialontologies.org/ontology/core/Core/Agreement"/>
        <rdfs:comment xml:lang="en">Specifies the agreement related to the maintenance work order record. This property establishes a connection between a maintenance work order and the agreement associated with it.</rdfs:comment>
        <rdfs:label xml:lang="en">related agreement</rdfs:label>
    </owl:ObjectProperty>
    


    <!-- https://w3id.org/def/bm2o#relatedCommercialService -->


    <owl:ObjectProperty rdf:about="https://w3id.org/def/bm2o#relatedCommercialService">
        <rdfs:domain rdf:resource="https://spec.industrialontologies.org/ontology/core/Core/Agreement"/>
        <rdfs:range rdf:resource="https://spec.industrialontologies.org/ontology/core/Core/CommercialService"/>
        <rdfs:comment xml:lang="en">This property establishes a connection between an agreement and the commercial service associated with it.</rdfs:comment>
        <rdfs:label xml:lang="en">related commercial service</rdfs:label>
    </owl:ObjectProperty>
    


    <!-- https://w3id.org/def/bm2o#relatedCustomer -->


    <owl:ObjectProperty rdf:about="https://w3id.org/def/bm2o#relatedCustomer">
        <rdfs:domain rdf:resource="https://spec.industrialontologies.org/ontology/core/Core/Agreement"/>
        <rdfs:range rdf:resource="https://spec.industrialontologies.org/ontology/core/Core/Customer"/>
        <rdfs:comment xml:lang="en">This property establishes a connection between an agreement and the customer associated with it.</rdfs:comment>
        <rdfs:label xml:lang="en">related customer</rdfs:label>
    </owl:ObjectProperty>
    


    <!-- https://w3id.org/def/bm2o#relatedEquipment -->


    <owl:ObjectProperty rdf:about="https://w3id.org/def/bm2o#relatedEquipment">
        <rdfs:domain rdf:resource="https://spec.industrialontologies.org/ontology/maintenance/MaintenanceReferenceOntology/MaintenanceProcess"/>
        <rdfs:range rdf:resource="https://brickschema.org/schema/1.1/Brick#Equipment"/>
        <rdfs:comment xml:lang="en">Specifies the equipment related to a maintenance process</rdfs:comment>
        <rdfs:label xml:lang="en">related equipment</rdfs:label>
    </owl:ObjectProperty>
    


    <!-- https://w3id.org/def/bm2o#relatedMaintenanceProcess -->


    <owl:ObjectProperty rdf:about="https://w3id.org/def/bm2o#relatedMaintenanceProcess">
        <rdfs:domain rdf:resource="https://spec.industrialontologies.org/ontology/maintenance/MaintenanceReferenceOntology/MaintenanceWorkOrderRecord"/>
        <rdfs:range rdf:resource="https://spec.industrialontologies.org/ontology/maintenance/MaintenanceReferenceOntology/MaintenanceProcess"/>
        <rdfs:comment xml:lang="en">Links a maintenance work order record to the specific maintenance process it is associated with.</rdfs:comment>
        <rdfs:label xml:lang="en">related maintenance process</rdfs:label>
    </owl:ObjectProperty>
    


    <!-- https://w3id.org/def/bm2o#relatedServiceLevelAgreement -->


    <owl:ObjectProperty rdf:about="https://w3id.org/def/bm2o#relatedServiceLevelAgreement">
        <rdfs:domain rdf:resource="https://spec.industrialontologies.org/ontology/core/Core/Agreement"/>
        <rdfs:range rdf:resource="https://w3id.org/def/bm2o#ServiceLevelAgreement"/>
        <rdfs:comment xml:lang="en">Specifies the service level agreement related to an agreement</rdfs:comment>
        <rdfs:label xml:lang="en">related service level agreement</rdfs:label>
    </owl:ObjectProperty>
    


    <!-- https://w3id.org/def/bm2o#relatedServiceProvider -->


    <owl:ObjectProperty rdf:about="https://w3id.org/def/bm2o#relatedServiceProvider">
        <rdfs:domain rdf:resource="https://spec.industrialontologies.org/ontology/core/Core/Agreement"/>
        <rdfs:range rdf:resource="https://spec.industrialontologies.org/ontology/core/Core/ServiceProvider"/>
        <rdfs:comment xml:lang="en">Specifies the service provider associated with an agreement. This property links an agreement to the service provider responsible for providing the specified services.</rdfs:comment>
        <rdfs:label xml:lang="en">related service provider</rdfs:label>
    </owl:ObjectProperty>
    


    <!-- 
    ///////////////////////////////////////////////////////////////////////////////////////
    //
    // Data properties
    //
    ///////////////////////////////////////////////////////////////////////////////////////
     -->


    


    <!-- https://w3id.org/def/bm2o#criticalLevel -->


    <owl:DatatypeProperty rdf:about="https://w3id.org/def/bm2o#criticalLevel">
        <rdfs:domain rdf:resource="https://spec.industrialontologies.org/ontology/maintenance/MaintenanceReferenceOntology/MaintenanceWorkOrderRecord"/>
        <rdfs:range rdf:resource="http://www.w3.org/2001/XMLSchema#integer"/>
        <rdfs:comment xml:lang="en">The critical level of the maintenance process.</rdfs:comment>
        <rdfs:label xml:lang="en">critical level</rdfs:label>
    </owl:DatatypeProperty>
    


    <!-- https://w3id.org/def/bm2o#customerCode -->


    <owl:DatatypeProperty rdf:about="https://w3id.org/def/bm2o#customerCode">
        <rdfs:domain rdf:resource="https://w3id.org/def/bm2o#ServiceLevelAgreement"/>
        <rdfs:range rdf:resource="http://www.w3.org/2001/XMLSchema#string"/>
        <rdfs:comment xml:lang="en">The customer code of the service level agreement.</rdfs:comment>
        <rdfs:label xml:lang="en">customer code</rdfs:label>
    </owl:DatatypeProperty>
    


    <!-- https://w3id.org/def/bm2o#description -->


    <owl:DatatypeProperty rdf:about="https://w3id.org/def/bm2o#description">
        <rdfs:domain rdf:resource="https://spec.industrialontologies.org/ontology/maintenance/MaintenanceReferenceOntology/MaintenanceWorkOrderRecord"/>
        <rdfs:range rdf:resource="http://www.w3.org/2001/XMLSchema#string"/>
        <rdfs:comment xml:lang="en">The description of the maintenance process.</rdfs:comment>
        <rdfs:label xml:lang="en">description</rdfs:label>
    </owl:DatatypeProperty>
    


    <!-- https://w3id.org/def/bm2o#estimatedInterventionDuration -->


    <owl:DatatypeProperty rdf:about="https://w3id.org/def/bm2o#estimatedInterventionDuration">
        <rdfs:domain rdf:resource="https://w3id.org/def/bm2o#ServiceLevelAgreement"/>
        <rdfs:range rdf:resource="http://www.w3.org/2001/XMLSchema#double"/>
        <rdfs:comment xml:lang="en">The estimated time to intervention of any maintenance process covered by the service level agreement.</rdfs:comment>
        <rdfs:label xml:lang="en">estimated intervention duration</rdfs:label>
    </owl:DatatypeProperty>
    


    <!-- https://w3id.org/def/bm2o#estimatedInterventionDurationUnit -->


    <owl:DatatypeProperty rdf:about="https://w3id.org/def/bm2o#estimatedInterventionDurationUnit">
        <rdfs:domain rdf:resource="https://w3id.org/def/bm2o#ServiceLevelAgreement"/>
        <rdfs:range rdf:resource="http://www.w3.org/2001/XMLSchema#string"/>
        <rdfs:comment xml:lang="en">The unit in which is defined the estimated intervention duration (a double) of any maintenance process covered by the service level agreement.</rdfs:comment>
        <rdfs:label xml:lang="en">estimated intervention duration unit</rdfs:label>
    </owl:DatatypeProperty>
    


    <!-- https://w3id.org/def/bm2o#label -->


    <owl:DatatypeProperty rdf:about="https://w3id.org/def/bm2o#label">
        <rdfs:domain rdf:resource="https://spec.industrialontologies.org/ontology/core/Core/Customer"/>
        <rdfs:domain rdf:resource="https://spec.industrialontologies.org/ontology/core/Core/ServiceProvider"/>
        <rdfs:range rdf:resource="http://www.w3.org/2001/XMLSchema#string"/>
        <rdfs:comment xml:lang="en">The label of the service provider.</rdfs:comment>
        <rdfs:label xml:lang="en">label</rdfs:label>
    </owl:DatatypeProperty>
    


    <!-- https://w3id.org/def/bm2o#maxTimeToIntervention -->


    <owl:DatatypeProperty rdf:about="https://w3id.org/def/bm2o#maxTimeToIntervention">
        <rdfs:domain rdf:resource="https://w3id.org/def/bm2o#ServiceLevelAgreement"/>
        <rdfs:range rdf:resource="http://www.w3.org/2001/XMLSchema#double"/>
        <rdfs:comment xml:lang="en">The maximum time to intervention of any maintenance process covered by the service level agreement.</rdfs:comment>
        <rdfs:label xml:lang="en">max time to intervention</rdfs:label>
    </owl:DatatypeProperty>
    


    <!-- https://w3id.org/def/bm2o#maxTimeToInterventionUnit -->


    <owl:DatatypeProperty rdf:about="https://w3id.org/def/bm2o#maxTimeToInterventionUnit">
        <rdfs:domain rdf:resource="https://w3id.org/def/bm2o#ServiceLevelAgreement"/>
        <rdfs:range rdf:resource="http://www.w3.org/2001/XMLSchema#string"/>
        <rdfs:comment xml:lang="en">The unit in which is defined the maximum time to intervention (a double) of any maintenance process covered by the service level agreement.</rdfs:comment>
        <rdfs:label xml:lang="en">max time to intervention unit</rdfs:label>
    </owl:DatatypeProperty>
    


    <!-- https://w3id.org/def/bm2o#maxTimeToRecovery -->


    <owl:DatatypeProperty rdf:about="https://w3id.org/def/bm2o#maxTimeToRecovery">
        <rdfs:domain rdf:resource="https://w3id.org/def/bm2o#ServiceLevelAgreement"/>
        <rdfs:range rdf:resource="http://www.w3.org/2001/XMLSchema#double"/>
        <rdfs:comment xml:lang="en">The maximum time to recovery of any maintenance process covered by the service level agreement.</rdfs:comment>
        <rdfs:label xml:lang="en">max time to recovery</rdfs:label>
    </owl:DatatypeProperty>
    


    <!-- https://w3id.org/def/bm2o#maxTimeToRecoveryUnit -->


    <owl:DatatypeProperty rdf:about="https://w3id.org/def/bm2o#maxTimeToRecoveryUnit">
        <rdfs:domain rdf:resource="https://w3id.org/def/bm2o#ServiceLevelAgreement"/>
        <rdfs:range rdf:resource="http://www.w3.org/2001/XMLSchema#string"/>
        <rdfs:comment xml:lang="en">The unit in which is defined the maximum time to recovery (a double) of any maintenance process covered by the service level agreement.</rdfs:comment>
        <rdfs:label xml:lang="en">max time to recovery unit</rdfs:label>
    </owl:DatatypeProperty>
    


    <!-- https://w3id.org/def/bm2o#serviceProviderCode -->


    <owl:DatatypeProperty rdf:about="https://w3id.org/def/bm2o#serviceProviderCode">
        <rdfs:domain rdf:resource="https://spec.industrialontologies.org/ontology/maintenance/MaintenanceReferenceOntology/MaintenanceWorkOrderRecord"/>
        <rdfs:range rdf:resource="http://www.w3.org/2001/XMLSchema#string"/>
        <rdfs:comment xml:lang="en">The service provider code of a maintenance process.</rdfs:comment>
        <rdfs:label xml:lang="en">service provider code</rdfs:label>
    </owl:DatatypeProperty>
    


    <!-- https://w3id.org/def/bm2o#technicalReason -->


    <owl:DatatypeProperty rdf:about="https://w3id.org/def/bm2o#technicalReason">
        <rdfs:domain rdf:resource="https://spec.industrialontologies.org/ontology/maintenance/MaintenanceReferenceOntology/MaintenanceWorkOrderRecord"/>
        <rdfs:range rdf:resource="http://www.w3.org/2001/XMLSchema#string"/>
        <rdfs:comment xml:lang="en">The technical reason of a maintenance process.</rdfs:comment>
        <rdfs:label xml:lang="en">technical reason</rdfs:label>
    </owl:DatatypeProperty>
    


    <!-- https://w3id.org/def/bm2o#topic -->


    <owl:DatatypeProperty rdf:about="https://w3id.org/def/bm2o#topic">
        <rdfs:domain rdf:resource="https://spec.industrialontologies.org/ontology/maintenance/MaintenanceReferenceOntology/MaintenanceWorkOrderRecord"/>
        <rdfs:range rdf:resource="http://www.w3.org/2001/XMLSchema#string"/>
        <rdfs:comment xml:lang="en">The topic of a maintenance process.</rdfs:comment>
        <rdfs:label xml:lang="en">topic</rdfs:label>
    </owl:DatatypeProperty>
    


    <!-- https://w3id.org/def/bm2o#workType -->


    <owl:DatatypeProperty rdf:about="https://w3id.org/def/bm2o#workType">
        <rdfs:domain rdf:resource="https://spec.industrialontologies.org/ontology/maintenance/MaintenanceReferenceOntology/MaintenanceWorkOrderRecord"/>
        <rdfs:range rdf:resource="http://www.w3.org/2001/XMLSchema#string"/>
        <rdfs:comment xml:lang="en">The type of work needed for a maintenance process.</rdfs:comment>
        <rdfs:label xml:lang="en">work type</rdfs:label>
    </owl:DatatypeProperty>
    


    <!-- 
    ///////////////////////////////////////////////////////////////////////////////////////
    //
    // Classes
    //
    ///////////////////////////////////////////////////////////////////////////////////////
     -->


    


    <!-- https://brickschema.org/schema/1.1/Brick#Equipment -->


    <rdf:Description rdf:about="https://brickschema.org/schema/1.1/Brick#Equipment">
        <owl:equivalentClass rdf:resource="https://spec.industrialontologies.org/ontology/core/Core/MaintainableMaterialItem"/>
    </rdf:Description>
    


    <!-- https://w3id.org/def/bm2o#Address -->


    <owl:Class rdf:about="https://w3id.org/def/bm2o#Address">
        <rdfs:comment xml:lang="en">Descriptin of a physical address</rdfs:comment>
        <rdfs:label xml:lang="en">Address</rdfs:label>
    </owl:Class>
    


    <!-- https://w3id.org/def/bm2o#Adjust -->


    <owl:Class rdf:about="https://w3id.org/def/bm2o#Adjust">
        <rdfs:subClassOf rdf:resource="https://spec.industrialontologies.org/ontology/maintenance/MaintenanceReferenceOntology/MaintenanceActivity"/>
        <rdfs:comment xml:lang="en">Maintenance activity that consists in setting a variable control mechanism to the correct specification to retain or restore the function of a maintainable item.</rdfs:comment>
        <rdfs:label xml:lang="en">Adjust</rdfs:label>
    </owl:Class>
    


    <!-- https://w3id.org/def/bm2o#Collectivity -->


    <owl:Class rdf:about="https://w3id.org/def/bm2o#Collectivity">
        <rdfs:subClassOf rdf:resource="https://spec.industrialontologies.org/ontology/core/Core/Customer"/>
        <rdfs:comment xml:lang="en">Organization of legal organizations.</rdfs:comment>
        <rdfs:label xml:lang="en">Collectivity</rdfs:label>
    </owl:Class>
    


    <!-- https://w3id.org/def/bm2o#ElevatorServiceProvider -->


    <owl:Class rdf:about="https://w3id.org/def/bm2o#ElevatorServiceProvider">
        <rdfs:subClassOf rdf:resource="https://spec.industrialontologies.org/ontology/core/Core/ServiceProvider"/>
        <rdfs:comment xml:lang="en">Person or organization which provides services related to elevators.</rdfs:comment>
        <rdfs:label xml:lang="en">Elevator Service Provider</rdfs:label>
    </owl:Class>
    


    <!-- https://w3id.org/def/bm2o#HeatingServiceProvider -->


    <owl:Class rdf:about="https://w3id.org/def/bm2o#HeatingServiceProvider">
        <rdfs:subClassOf rdf:resource="https://spec.industrialontologies.org/ontology/core/Core/ServiceProvider"/>
        <rdfs:comment xml:lang="en">Person or organization which provides services related to heating.</rdfs:comment>
        <rdfs:label xml:lang="en">Heating Service Provider</rdfs:label>
    </owl:Class>
    


    <!-- https://w3id.org/def/bm2o#Inspect -->


    <owl:Class rdf:about="https://w3id.org/def/bm2o#Inspect">
        <rdfs:subClassOf rdf:resource="https://spec.industrialontologies.org/ontology/maintenance/MaintenanceReferenceOntology/MaintenanceActivity"/>
        <rdfs:comment xml:lang="en">Maintenance activity that consists in inspecting some component of a maintainable item to retain its function.</rdfs:comment>
        <rdfs:label xml:lang="en">Inspect</rdfs:label>
    </owl:Class>
    


    <!-- https://w3id.org/def/bm2o#LandscapingServiceProvider -->


    <owl:Class rdf:about="https://w3id.org/def/bm2o#LandscapingServiceProvider">
        <rdfs:subClassOf rdf:resource="https://spec.industrialontologies.org/ontology/core/Core/ServiceProvider"/>
        <rdfs:comment xml:lang="en">Person or organization which provides services related to landscaping.</rdfs:comment>
        <rdfs:label xml:lang="en">Landscaping Service Provider</rdfs:label>
    </owl:Class>
    


    <!-- https://w3id.org/def/bm2o#MultiserviceProvider -->


    <owl:Class rdf:about="https://w3id.org/def/bm2o#MultiserviceProvider">
        <rdfs:subClassOf rdf:resource="https://spec.industrialontologies.org/ontology/core/Core/ServiceProvider"/>
        <rdfs:comment xml:lang="en">Person or organization which provides multiple building-related services.</rdfs:comment>
        <rdfs:label xml:lang="en">Multiservice Provider</rdfs:label>
    </owl:Class>
    


    <!-- https://w3id.org/def/bm2o#PaintingServiceProvider -->


    <owl:Class rdf:about="https://w3id.org/def/bm2o#PaintingServiceProvider">
        <rdfs:subClassOf rdf:resource="https://spec.industrialontologies.org/ontology/core/Core/ServiceProvider"/>
        <rdfs:comment xml:lang="en">Person or organization which provides services related to painting.</rdfs:comment>
        <rdfs:label xml:lang="en">Painting Service Provider</rdfs:label>
    </owl:Class>
    


    <!-- https://w3id.org/def/bm2o#PlumbingServiceProvider -->


    <owl:Class rdf:about="https://w3id.org/def/bm2o#PlumbingServiceProvider">
        <rdfs:subClassOf rdf:resource="https://spec.industrialontologies.org/ontology/core/Core/ServiceProvider"/>
        <rdfs:comment xml:lang="en">Person or organization which provides services related to plumbing.</rdfs:comment>
        <rdfs:label xml:lang="en">Plumbing Service Provider</rdfs:label>
    </owl:Class>
    


    <!-- https://w3id.org/def/bm2o#PropertyManager -->


    <owl:Class rdf:about="https://w3id.org/def/bm2o#PropertyManager">
        <rdfs:subClassOf rdf:resource="https://spec.industrialontologies.org/ontology/core/Core/Customer"/>
        <rdfs:comment xml:lang="en">Person or organization hired to oversee the day-to-day operations of a unit of real estate.</rdfs:comment>
        <rdfs:label xml:lang="en">Property Manager</rdfs:label>
    </owl:Class>
    


    <!-- https://w3id.org/def/bm2o#Repair -->


    <owl:Class rdf:about="https://w3id.org/def/bm2o#Repair">
        <rdfs:subClassOf rdf:resource="https://spec.industrialontologies.org/ontology/maintenance/MaintenanceReferenceOntology/MaintenanceActivity"/>
        <rdfs:comment xml:lang="en">Maintenance activity that consists in repairing some component of a maintainable item to retain or restore its function.</rdfs:comment>
        <rdfs:label xml:lang="en">Repair</rdfs:label>
    </owl:Class>
    


    <!-- https://w3id.org/def/bm2o#Replace -->


    <owl:Class rdf:about="https://w3id.org/def/bm2o#Replace">
        <rdfs:subClassOf rdf:resource="https://spec.industrialontologies.org/ontology/maintenance/MaintenanceReferenceOntology/MaintenanceActivity"/>
        <rdfs:comment xml:lang="en">Maintenance activity that consists in replacing some component of a maintainable item to retain or restore its function.</rdfs:comment>
        <rdfs:label xml:lang="en">Replace</rdfs:label>
    </owl:Class>
    


    <!-- https://w3id.org/def/bm2o#ServiceLevelAgreement -->


    <owl:Class rdf:about="https://w3id.org/def/bm2o#ServiceLevelAgreement">
        <rdfs:comment xml:lang="en">Contract between a service provider and its customers that documents what services the provider will furnish and defines the service standards the provider is obligated to meet.</rdfs:comment>
        <rdfs:label xml:lang="en">Service Level Agreement</rdfs:label>
    </owl:Class>
    


    <!-- https://w3id.org/def/bm2o#Tertiary -->


    <owl:Class rdf:about="https://w3id.org/def/bm2o#Tertiary">
        <rdfs:subClassOf rdf:resource="https://spec.industrialontologies.org/ontology/core/Core/Customer"/>
        <rdfs:comment xml:lang="en">Tertiary industries or companies are involved in providing services, rather than the production of raw materials or manufacturing. (Source: ldoce)</rdfs:comment>
        <rdfs:label xml:lang="en">Tertiary</rdfs:label>
    </owl:Class>
    


    <!-- https://w3id.org/def/bm2o#VentilationServiceProvider -->


    <owl:Class rdf:about="https://w3id.org/def/bm2o#VentilationServiceProvider">
        <rdfs:subClassOf rdf:resource="https://spec.industrialontologies.org/ontology/core/Core/ServiceProvider"/>
        <rdfs:comment xml:lang="en">Person or organization which provides services related to ventilation.</rdfs:comment>
        <rdfs:label xml:lang="en">Ventilation Service Provider</rdfs:label>
    </owl:Class>
</rdf:RDF>



<!-- Generated by the OWL API (version 5.1.18) https://github.com/owlcs/owlapi/ -->


